James C - start of massive (but formatting-only) adjustments

isabelle/DeBruijnEnvironment.thy
@@ -4,182 +4,181 @@ begin
 
 datatype 'a env = DBEnv "'a list"
 
-primrec env_size :: "'a env => nat"
-where "env_size (DBEnv as) = length as"
+primrec env_size :: "'a env \<Rightarrow> nat" where 
+  "env_size (DBEnv as) = length as"
 
-definition empty_env :: "'a env"
-where "empty_env = DBEnv []"
+definition empty_env :: "'a env" where 
+  "empty_env = DBEnv []"
 
-fun is_in :: "var => 'a env => bool" (infix "in" 65)
-where "is_in (DBVar n) (DBEnv as) = (n <= length as)"
+fun is_in :: "var \<Rightarrow> 'a env \<Rightarrow> bool" (infix "in" 65) where 
+  "is_in (DBVar n) (DBEnv as) = (n \<le> length as)"
 
-fun lookup' :: "'a list => nat => 'a option"
-where "lookup' [] n = None"
-    | "lookup' (a # as) 0 = Some a"
-    | "lookup' (a # as) (Suc n) = lookup' as n"
+fun lookup' :: "'a list \<Rightarrow> nat \<Rightarrow> 'a option" where 
+  "lookup' [] n = None"
+| "lookup' (a # as) 0 = Some a"
+| "lookup' (a # as) (Suc n) = lookup' as n"
 
-fun lookup :: "'a env => var => 'a option"
-where "lookup (DBEnv as) (DBVar n) = lookup' as n"
+fun lookup :: "'a env \<Rightarrow> var \<Rightarrow> 'a option" where 
+  "lookup (DBEnv as) (DBVar n) = lookup' as n"
 
-fun extend_at' :: "nat => 'a list => 'a => 'a list"
-where "extend_at' 0 as a' = a' # as"
-    | "extend_at' (Suc n) [] a' = undefined"
-    | "extend_at' (Suc n) (a # as) a' = a # extend_at' n as a'"
+fun extend_at' :: "nat \<Rightarrow> 'a list \<Rightarrow> 'a \<Rightarrow> 'a list" where 
+  "extend_at' 0 as a' = a' # as"
+| "extend_at' (Suc n) [] a' = undefined"
+| "extend_at' (Suc n) (a # as) a' = a # extend_at' n as a'"
 
-fun extend_at :: "var => 'a env => 'a => 'a env"
-where "extend_at (DBVar n) (DBEnv as) a' = DBEnv (extend_at' n as a')"
+fun extend_at :: "var \<Rightarrow> 'a env \<Rightarrow> 'a \<Rightarrow> 'a env" where 
+  "extend_at (DBVar n) (DBEnv as) a' = DBEnv (extend_at' n as a')"
 
-abbreviation extend :: "'a env => 'a => 'a env"
-where "extend == extend_at first"
+abbreviation extend :: "'a env \<Rightarrow> 'a \<Rightarrow> 'a env" where 
+  "extend \<equiv> extend_at first"
 
-fun append :: "'a env => 'a env => 'a env" (infix "+++" 65)
-where "DBEnv a +++ DBEnv b = DBEnv (a @ b)"
+fun append :: "'a env \<Rightarrow> 'a env \<Rightarrow> 'a env" (infix "+++" 65) where 
+  "DBEnv a +++ DBEnv b = DBEnv (a @ b)"
 
-primrec env_map :: "('a => 'b) => 'a env => 'b env"
-where "env_map f (DBEnv n) = DBEnv (map f n)" 
+primrec env_map :: "('a \<Rightarrow> 'b) \<Rightarrow> 'a env \<Rightarrow> 'b env" where 
+  "env_map f (DBEnv n) = DBEnv (map f n)" 
 
-fun update' :: "'a list => nat => 'a => 'a list"
-where "update' [] n a = undefined"
-    | "update' (b # bs) 0 a = a # bs"
-    | "update' (b # bs) (Suc n) a = b # update' bs n a"
+fun update' :: "'a list \<Rightarrow> nat \<Rightarrow> 'a \<Rightarrow> 'a list" where 
+  "update' [] n a = undefined"
+| "update' (b # bs) 0 a = a # bs"
+| "update' (b # bs) (Suc n) a = b # update' bs n a"
 
-fun update :: "'a env => var => 'a => 'a env"
-where "update (DBEnv e) (DBVar v) a = DBEnv (update' e v a)" 
+fun update :: "'a env \<Rightarrow> var \<Rightarrow> 'a \<Rightarrow> 'a env" where 
+  "update (DBEnv e) (DBVar v) a = DBEnv (update' e v a)" 
 
 lemma [simp]: "first in gam"
-by (induction gam, simp add: first_def)
+  by (induction gam) (simp add: first_def)
 
-lemma [simp]: "x <= length list ==> length (extend_at' x list y) = Suc (length list)"
-by (induction x list y rule: extend_at'.induct, simp_all)
+lemma [simp]: "x \<le> length list \<Longrightarrow> length (extend_at' x list y) = Suc (length list)"
+  by (induction x list y rule: extend_at'.induct) simp_all
 
-lemma [simp]: "x in gam ==> n in gam ==> next n in extend_at x gam y"
-by (induction gam, induction x, induction n, simp)
+lemma [simp]: "x in gam \<Longrightarrow> n in gam \<Longrightarrow> next n in extend_at x gam y"
+  by (induction gam, induction x, induction n) simp
 
-lemma [simp]: "n in g2 ==> (next_by (env_size g1) n) in (g1 +++ g2)"
-by (induction g1, induction g2, induction n, simp)
+lemma [simp]: "n in g2 \<Longrightarrow> (next_by (env_size g1) n) in (g1 +++ g2)"
+  by (induction g1, induction g2, induction n) simp
 
-lemma [simp]: "x in e ==> env_size (extend_at x e y) = Suc (env_size e)"
-by (induction x e y rule: extend_at.induct, simp)
+lemma [simp]: "x in e \<Longrightarrow> env_size (extend_at x e y) = Suc (env_size e)"
+  by (induction x e y rule: extend_at.induct) simp
 
 lemma [simp]: "env_size empty_env = 0"
-by (simp add: empty_env_def)
+  by (simp add: empty_env_def)
 
-lemma [elim!]: "env_size gam = 0 ==> gam = empty_env"
-by (induction gam, simp add: empty_env_def)
+lemma [elim!]: "env_size gam = 0 \<Longrightarrow> gam = empty_env"
+  by (induction gam) (simp add: empty_env_def)
 
-lemma [elim!]: "env_size gam = Suc n ==> EX gam' t. gam = extend gam' t & env_size gam' = n"
-proof (induction gam)
-case (DBEnv g)
-  thus ?case
-  proof (cases g, simp)
-  case (Cons t g')
-    hence "DBEnv g = extend (DBEnv g') t" by (simp add: first_def)
-    moreover from DBEnv Cons have "env_size (DBEnv g') = n" by simp
-    ultimately show ?thesis by auto
+lemma [elim!]: "env_size gam = Suc n \<Longrightarrow> \<exists>gam' t. gam = extend gam' t \<and> env_size gam' = n"
+  proof (induction gam)
+  case (DBEnv g)
+    thus ?case
+      proof (cases g, simp)
+      case (Cons t g')
+        hence "DBEnv g = extend (DBEnv g') t" by (simp add: first_def)
+        moreover from DBEnv Cons have "env_size (DBEnv g') = n" by simp
+        ultimately show ?thesis by auto
+      qed
   qed
-qed
 
 lemma [simp]: "env_size (e1 +++ e2) = env_size e1 + env_size e2"
-by (induction e1, induction e2, simp)
+  by (induction e1, induction e2) simp
 
 lemma [simp]: "empty_env +++ e = e"
-by (induction e, simp add: empty_env_def)
+  by (induction e) (simp add: empty_env_def)
 
 lemma [simp]: "e +++ empty_env = e"
-by (induction e, simp add: empty_env_def)
+  by (induction e) (simp add: empty_env_def)
 
 lemma [simp]: "extend e t +++ e' = extend (e +++ e') t"
-by (induction e, induction e', simp add: first_def)
+  by (induction e, induction e') (simp add: first_def)
 
 lemma [simp]: "lookup empty_env x = None"
-by (cases x, simp add: empty_env_def)
+  by (cases x) (simp add: empty_env_def)
 
-lemma [simp]: "n <= length l ==> length (extend_at' n l a) = Suc (length l)"
-by (induction n l a rule: extend_at'.induct, simp_all)
+lemma [simp]: "n \<le> length l \<Longrightarrow> length (extend_at' n l a) = Suc (length l)"
+  by (induction n l a rule: extend_at'.induct) simp_all
 
-lemma [simp]: "n <= length l ==> lookup' (extend_at' n l t) x = 
-                  (if x < n then lookup' l x else if x > n then lookup' l (x - 1) else Some t)"
-proof (induction n l t arbitrary: x rule: extend_at'.induct)
-case 1
-  thus ?case by (cases x, simp_all)
-next case 2
-  thus ?case by simp
-next case 3
-  thus ?case
-  proof (cases x)
-  case 0
-    thus ?thesis by simp
-  next case (Suc x')
-    with 3 show ?thesis by (cases x', simp_all)
+lemma [simp]: "n \<le> length l \<Longrightarrow> lookup' (extend_at' n l t) x = 
+    (if x < n then lookup' l x else if x > n then lookup' l (x - 1) else Some t)"
+  proof (induction n l t arbitrary: x rule: extend_at'.induct)
+  case 1
+    thus ?case by (cases x) simp_all
+  next case 2
+    thus ?case by simp
+  next case 3
+    thus ?case
+      proof (cases x)
+      case 0
+        thus ?thesis by simp
+      next case (Suc x')
+        with 3 show ?thesis by (cases x') simp_all
+      qed
   qed
-qed
 
-lemma [simp]: "n in gam ==> x ~= n ==> 
-          lookup (extend_at n gam t) x = lookup gam (subr n x)"
-by (induction gam, induction n, induction x, simp)
+lemma [simp]: "n in gam \<Longrightarrow> x \<noteq> n \<Longrightarrow> lookup (extend_at n gam t) x = lookup gam (subr n x)"
+  by (induction gam, induction n, induction x) simp
 
-lemma [simp]: "n in gam ==> lookup (extend_at n gam t) n = Some t"
-by (induction gam, induction n, simp)
+lemma [simp]: "n in gam \<Longrightarrow> lookup (extend_at n gam t) n = Some t"
+  by (induction gam, induction n) simp
 
-lemma [simp]: "n in gam ==> lookup gam x = Some t ==> 
-         lookup (extend_at n gam t') (incr n x) = Some t"
-by (induction gam, induction n, induction x, simp)
+lemma [simp]: "n in gam \<Longrightarrow> lookup gam x = Some t \<Longrightarrow> 
+    lookup (extend_at n gam t') (incr n x) = Some t"
+  by (induction gam, induction n, induction x) simp
 
-lemma [simp]: "n <= length l ==> m <= n ==> 
-          extend_at' m (extend_at' n l a) b = extend_at' (Suc n) (extend_at' m l b) a"
-proof (induction n l a arbitrary: m rule: extend_at'.induct)
-case 1
-  thus ?case by simp
-next case 2
-  thus ?case by simp
-next case 3
-  thus ?case by (cases m, simp_all)
-qed
+lemma [simp]: "n \<le> length l \<Longrightarrow> m \<le> n \<Longrightarrow> 
+    extend_at' m (extend_at' n l a) b = extend_at' (Suc n) (extend_at' m l b) a"
+  proof (induction n l a arbitrary: m rule: extend_at'.induct)
+  case 1
+    thus ?case by simp
+  next case 2
+    thus ?case by simp
+  next case 3
+    thus ?case by (cases m) simp_all
+  qed
 
 lemma [simp]: "extend_at' (n + length e1) (e1 @ e2) t = e1 @ extend_at' n e2 t"
-by (induction e1, simp_all)
+  by (induction e1) simp_all
 
 lemma [simp]: "extend_at (next_by (env_size e1) n) (e1 +++ e2) t = e1 +++ extend_at n e2 t"
-by (induction e1, induction e2, induction n, simp)
+  by (induction e1, induction e2, induction n) simp
 
-lemma [simp]: "n in gam ==> canswap m n ==>
-        extend_at m (extend_at n gam a) b = extend_at (next n) (extend_at m gam b) a"
-by (induction gam, induction n, induction m, simp)
+lemma [simp]: "n in gam \<Longrightarrow> canswap m n \<Longrightarrow> 
+    extend_at m (extend_at n gam a) b = extend_at (next n) (extend_at m gam b) a"
+  by (induction gam, induction n, induction m) simp
 
-lemma [simp]: "n in gam ==> canswap m n ==> m in gam"
-by (induction gam, induction n, induction m, simp)
+lemma [simp]: "n in gam \<Longrightarrow> canswap m n \<Longrightarrow> m in gam"
+  by (induction gam, induction n, induction m) simp
 
 lemma [simp]: "env_map f empty_env = empty_env"
-by (simp add: empty_env_def)
+  by (simp add: empty_env_def)
 
-lemma [simp]: "lookup' env x = Some v ==> lookup' (map f env) x = Some (f v)"
-by (induction env x rule: lookup'.induct, simp_all)
+lemma [simp]: "lookup' env x = Some v \<Longrightarrow> lookup' (map f env) x = Some (f v)"
+  by (induction env x rule: lookup'.induct) simp_all
 
-lemma [simp]: "lookup env x = Some v ==> lookup (env_map f env) x = Some (f v)"
-by (induction env, induction x, simp)
+lemma [simp]: "lookup env x = Some v \<Longrightarrow> lookup (env_map f env) x = Some (f v)"
+  by (induction env, induction x) simp
                 
-lemma [elim]: "inj f ==> lookup' (map f env) x = Some (f v) ==> lookup' env x = Some v"
-by (induction env x rule: lookup'.induct, simp, simp add: inj_on_def, fastforce) 
+lemma [elim]: "inj f \<Longrightarrow> lookup' (map f env) x = Some (f v) \<Longrightarrow> lookup' env x = Some v"
+  by (induction env x rule: lookup'.induct) (simp, simp add: inj_on_def, fastforce) 
 
-lemma [elim]: "inj f ==> lookup (env_map f env) x = Some (f v) ==> lookup env x = Some v"
-by (induction env, induction x, auto)
+lemma [elim]: "inj f \<Longrightarrow> lookup (env_map f env) x = Some (f v) \<Longrightarrow> lookup env x = Some v"
+  by (induction env, induction x) auto
 
-lemma [simp]: "n <= length env ==> extend_at' n (map f env) (f t) = map f (extend_at' n env t)" 
-by (induction n env t rule: extend_at'.induct, simp_all)
+lemma [simp]: "n \<le> length env \<Longrightarrow> extend_at' n (map f env) (f t) = map f (extend_at' n env t)" 
+  by (induction n env t rule: extend_at'.induct) simp_all
 
-lemma [simp]: "n in env ==> extend_at n (env_map f env) (f t) = env_map f (extend_at n env t)" 
-by (induction env, induction n, simp)
+lemma [simp]: "n in env \<Longrightarrow> extend_at n (env_map f env) (f t) = env_map f (extend_at n env t)" 
+  by (induction env, induction n) simp
 
-lemma [simp]: "n in env ==> n in env_map f env" 
-by (induction env, induction n, simp)
+lemma [simp]: "n in env \<Longrightarrow> n in env_map f env" 
+  by (induction env, induction n) simp
 
 lemma [simp]: "env_map f (env_map g env) = env_map (f o g) env"
-by (induction env, simp)
+  by (induction env) simp
 
-lemma [simp]: "lookup' (map f env) n = Some t ==> EX t'. t = f t'"
-by (induction env n rule: lookup'.induct, auto)
+lemma [simp]: "lookup' (map f env) n = Some t \<Longrightarrow> \<exists>t'. t = f t'"
+  by (induction env n rule: lookup'.induct) auto
 
-lemma [simp]: "lookup (env_map f env) n = Some t ==> EX t'. t = f t'"
-by (induction env, induction n, simp)
+lemma [simp]: "lookup (env_map f env) n = Some t \<Longrightarrow> \<exists>t'. t = f t'"
+  by (induction env, induction n) simp
 
 end
